theories/input_lang_callcc/logrel.v
@@ -1,7 +1,9 @@
 (** Logical relation for adequacy for the IO lang *)
 From Equations Require Import Equations.
 From gitrees Require Import gitree.
-From gitrees.input_lang Require Import lang interp.
+From gitrees.input_lang_callcc Require Import lang interp.
+Require Import gitrees.lang_generic_sem.
+Require Import Binding.Lib Binding.Set Binding.Env.
 
 Section logrel.
   Context {sz : nat}.
@@ -16,7 +18,7 @@ Section logrel.
 
   Canonical Structure exprO S := leibnizO (expr S).
   Canonical Structure valO S := leibnizO (val S).
-  Local Notation tyctx := (tyctx ty).
+  Canonical Structure ectxO S := leibnizO (ectx S).
 
   Notation "'WP' α {{ β , Φ } }" := (wp rs α notStuck ⊤ (λ β, Φ))
     (at level 20, α, Φ at level 200,
@@ -26,394 +28,531 @@ Section logrel.
     (at level 20, α, Φ at level 200,
      format "'WP'  α  {{  Φ  } }") : bi_scope.
 
-  Definition logrel_expr {S} V (α : IT) (e : expr S) : iProp :=
+  Definition logrel_nat {S} (βv : ITV) (v : val S) : iProp :=
+    (∃ n, βv ≡ RetV n ∧ ⌜v = LitV n⌝)%I.
+
+  Definition obs_ref {S} (α : IT) (e : expr S) : iProp :=
     (∀ (σ : stateO),
         has_substate σ -∗
         WP α {{ βv, ∃ m v σ', ⌜prim_steps e σ (Val v) σ' m⌝
-                         ∗ V βv v ∗ has_substate σ' }})%I.
-  Definition logrel_nat {S} (βv : ITV) (v : val S) : iProp :=
-    (∃ n, βv ≡ RetV n ∧ ⌜v = Lit n⌝)%I.
-  Definition logrel_arr {S} V1 V2 (βv : ITV) (vf : val S) : iProp :=
-    (∃ f, IT_of_V βv ≡ Fun f ∧ □ ∀ αv v, V1 αv v -∗ logrel_expr V2 (APP' (Fun f) (IT_of_V αv)) (App (Val vf) (Val v)))%I.
+                              ∗ logrel_nat βv v ∗ has_substate σ' }})%I.
 
-  Fixpoint logrel_val (τ : ty) {S} : ITV → (val S) → iProp
+  Definition HOM : ofe := @sigO (IT -n> IT) IT_hom.
+
+  Global Instance HOM_hom (κ : HOM) : IT_hom (`κ).
+  Proof.
+    apply (proj2_sig κ).
+  Qed.
+
+  Definition logrel_ectx {S} V (κ : HOM) (K : ectx S) : iProp :=
+    (□ ∀ (βv : ITV) (v : val S), V βv v -∗ obs_ref (`κ (IT_of_V βv)) (fill K (Val v)))%I.
+
+  Definition logrel_expr {S} V (α : IT) (e : expr S) : iProp :=
+    (∀ (κ : HOM) (K : ectx S),
+       logrel_ectx V κ K -∗ obs_ref (`κ α) (fill K e))%I.
+
+  Definition logrel_arr {S} V1 V2 (βv : ITV) (vf : val S) : iProp :=
+    (∃ f, IT_of_V βv ≡ Fun f ∧ □ ∀ αv v, V1 αv v -∗
+      logrel_expr V2 (APP' (Fun f) (IT_of_V αv)) (App (Val vf) (Val v)))%I.
+
+  Global Instance denot_cont_ne (κ : IT -n> IT) :
+    NonExpansive (λ x : IT, Tau (laterO_map κ (Next x))).
+  Proof.
+    solve_proper.
+  Qed.
+
+  Definition logrel_cont {S} V (βv : ITV) (v : val S) : iProp :=
+    (∃ (κ : HOM) K, (IT_of_V βv) ≡ (Fun (Next (λne x, Tau (laterO_map (`κ) (Next x)))))
+                            ∧ ⌜v = ContV K⌝
+                            ∧ □ logrel_ectx V κ K)%I.
+
+  Fixpoint logrel_val {S} (τ : ty) : ITV → (val S) → iProp
     := match τ with
        | Tnat => logrel_nat
        | Tarr τ1 τ2 => logrel_arr (logrel_val τ1) (logrel_val τ2)
+       | Tcont τ => logrel_cont (logrel_val τ)
        end.
 
-  Definition logrel (τ : ty) {S} : IT → (expr S) → iProp
+  Definition logrel {S} (τ : ty) : IT → (expr S) → iProp
     := logrel_expr (logrel_val τ).
+
+  #[export] Instance obs_ref_ne {S} :
+    NonExpansive2 (@obs_ref S).
+  Proof.
+    solve_proper.
+  Qed.
 
   #[export] Instance logrel_expr_ne {S} (V : ITV → val S → iProp) :
     NonExpansive2 V → NonExpansive2 (logrel_expr V).
-  Proof. solve_proper. Qed.
+  Proof.
+    solve_proper.
+  Qed.
+
   #[export] Instance logrel_nat_ne {S} : NonExpansive2 (@logrel_nat S).
-  Proof. solve_proper. Qed.
-  #[export] Instance logrel_val_ne (τ : ty) {S} : NonExpansive2 (@logrel_val τ S).
-  Proof. induction τ; simpl; solve_proper. Qed.
+  Proof.
+    solve_proper.
+  Qed.
+
+  #[export] Instance logrel_val_ne {S} (τ : ty) : NonExpansive2 (@logrel_val S τ).
+  Proof.
+    induction τ; simpl; solve_proper.
+  Qed.
+
+  #[export] Instance logrel_ectx_ne {S} (V : ITV → val S → iProp) :
+    NonExpansive2 V → NonExpansive2 (logrel_ectx V).
+  Proof.
+    solve_proper.
+  Qed.
+
+  #[export] Instance logrel_arr_ne {S} (V1 V2 : ITV → val S → iProp) :
+    NonExpansive2 V1 -> NonExpansive2 V2 → NonExpansive2 (logrel_arr V1 V2).
+  Proof.
+    solve_proper.
+  Qed.
+
+  #[export] Instance logrel_cont_ne {S} (V : ITV → val S → iProp) :
+    NonExpansive2 V -> NonExpansive2 (logrel_cont V).
+  Proof.
+    solve_proper.
+  Qed.
+
+  #[export] Instance obs_ref_proper {S} :
+    Proper ((≡) ==> (≡) ==> (≡)) (@obs_ref S).
+  Proof.
+    solve_proper.
+  Qed.
+
   #[export] Instance logrel_expr_proper {S} (V : ITV → val S → iProp) :
-    Proper ((≡) ==> (≡) ==> (≡)) V →
-    Proper ((≡) ==> (≡) ==> (≡)) (logrel_expr V).
-  Proof. solve_proper. Qed.
-  #[export] Instance logrel_val_proper (τ : ty) {S} :
-    Proper ((≡) ==> (≡) ==> (≡)) (@logrel_val τ S).
-  Proof. induction τ; simpl; solve_proper. Qed.
-  #[export] Instance logrel_persistent (τ : ty) {S} α v :
-    Persistent (@logrel_val τ S α v).
+    Proper ((≡) ==> (≡) ==> (≡)) V → Proper ((≡) ==> (≡) ==> (≡)) (logrel_expr V).
+  Proof.
+    solve_proper.
+  Qed.
+
+  #[export] Instance logrel_nat_proper {S} : Proper ((≡) ==> (≡) ==> (≡)) (@logrel_nat S).
+  Proof.
+    solve_proper.
+  Qed.
+
+  #[export] Instance logrel_val_proper {S} (τ : ty) : Proper ((≡) ==> (≡) ==> (≡)) (@logrel_val S τ).
+  Proof.
+    induction τ; simpl; solve_proper.
+  Qed.
+
+  #[export] Instance logrel_ectx_proper {S} (V : ITV → val S → iProp) :
+    Proper ((≡) ==> (≡) ==> (≡)) V → Proper ((≡) ==> (≡) ==> (≡)) (logrel_ectx V).
+  Proof.
+    solve_proper.
+  Qed.
+
+  #[export] Instance logrel_arr_proper {S} (V1 V2 : ITV → val S → iProp) :
+    Proper ((≡) ==> (≡) ==> (≡)) V1 -> Proper ((≡) ==> (≡) ==> (≡)) V2 → Proper ((≡) ==> (≡) ==> (≡)) (logrel_arr V1 V2).
+  Proof.
+    solve_proper.
+  Qed.
+
+  #[export] Instance logrel_cont_proper {S} (V : ITV → val S → iProp) :
+    Proper ((≡) ==> (≡) ==> (≡)) V -> Proper ((≡) ==> (≡) ==> (≡)) (logrel_cont V).
+  Proof.
+    solve_proper.
+  Qed.
+
+  #[export] Instance logrel_val_persistent {S} (τ : ty) α v :
+    Persistent (@logrel_val S τ α v).
   Proof.
     revert α v. induction τ=> α v; simpl.
     - unfold logrel_nat. apply _.
     - unfold logrel_arr. apply _.
+    - unfold logrel_cont. apply _.
   Qed.
 
-  Lemma logrel_bind {S} (f : IT → IT) (K : ectx S) `{!IT_hom f}
-    e α τ1 V2 `{!NonExpansive2 V2} :
-    ⊢ logrel_expr (logrel_val τ1) α e -∗
-      (∀ v βv, logrel_val τ1 βv v -∗
-                   logrel_expr V2 (f (IT_of_V βv)) (fill K (Val v))) -∗
-      logrel_expr V2 (f α) (fill K e).
+  #[export] Instance logrel_ectx_persistent {S} V κ K :
+    Persistent (@logrel_ectx S V κ K).
   Proof.
-    iIntros "H1 H2".
+    apply _.
+  Qed.
+
+  Lemma logrel_of_val {S} τ αv (v : val S) :
+    logrel_val τ αv v -∗ logrel τ (IT_of_V αv) (Val v).
+  Proof.
+    iIntros "H1". iIntros (κ K) "HK".
+    iIntros (σ) "Hs".
+    by iApply ("HK" $! αv v with "[$H1] [$Hs]").
+  Qed.
+
+  Lemma HOM_ccompose (f g : HOM)
+    : ∀ α, `f (`g α) = (`f ◎ `g) α.
+  Proof.
+    intro; reflexivity.
+  Qed.
+
+  Lemma logrel_bind {S} (f : HOM) (K : ectx S)
+    e α τ1 :
+    ⊢ logrel τ1 α e -∗
+      logrel_ectx (logrel_val τ1) f K -∗
+      obs_ref (`f α) (fill K e).
+  Proof.
+    iIntros "H1 #H2".
     iLöb as "IH" forall (α e).
     iIntros (σ) "Hs".
-    iApply wp_bind.
-    { solve_proper. }
-    iSpecialize ("H1" with "Hs").
-    iApply (wp_wand with "H1").
-    iIntros (αv). iDestruct 1 as ([m m'] v σ' Hsteps) "[H1 Hs]".
-    apply (prim_steps_ctx K) in Hsteps.
-    iSpecialize ("H2" with "H1 Hs").
-    iApply (wp_wand with "H2"). iModIntro.
-    iIntros (βv). iDestruct 1 as ([m2 m2'] v2 σ2' Hsteps2) "[H2 Hs]".
-    iExists (m + m2, m' + m2'),v2,σ2'. iFrame "H2 Hs".
-    iPureIntro. eapply (prim_steps_app (m,m') (m2,m2')); eauto.
+    iApply (wp_wand with "[H1 H2 Hs] []"); first iApply ("H1" with "[H2] [$Hs]").
+    - iIntros (βv v). iModIntro.
+      iIntros "#Hv".
+      by iApply "H2".
+    - iIntros (βv).
+      iIntros "?".
+      iModIntro.
+      iFrame.
   Qed.
 
-  Lemma logrel_of_val {S} αv (v : val S) V :
-    V αv v -∗ logrel_expr V (IT_of_V αv) (Val v).
+  Definition ssubst2_valid {S : Set}
+    (Γ : S -> ty)
+    (ss : @interp_scope F natO _ S)
+    (γ : S [⇒] ∅)
+    : iProp :=
+    (∀ x, □ logrel (Γ x) (ss x) (γ x))%I.
+
+  Definition logrel_valid {S : Set}
+    (Γ : S -> ty)
+    (e : expr S)
+    (α : @interp_scope F natO _ S -n> IT)
+    (τ : ty) : iProp :=
+    (□ ∀ (ss : @interp_scope F natO _ S)
+       (γ : S [⇒] ∅),
+       ssubst2_valid Γ ss γ → logrel τ (α ss) (bind γ e))%I.
+
+  Lemma compat_var {S : Set} (Γ : S -> ty) (x : S) :
+    ⊢ logrel_valid Γ (Var x) (interp_var x) (Γ x).
   Proof.
-    iIntros "H1". iIntros (σ) "Hs".
-    iApply wp_val.
-    iExists (0,0),v,σ. iFrame. iPureIntro.
-    by econstructor.
+    iModIntro.
+    iIntros (ss γ) "Hss".
+    iApply "Hss".
   Qed.
 
-  Lemma logrel_step_pure {S} (e' e : expr S) α V :
-    (∀ σ, prim_step e σ e' σ (0,0)) →
-    logrel_expr V α e' ⊢ logrel_expr V α e.
+  Lemma logrel_head_step_pure_ectx {S} n K (κ : HOM) (e' e : expr S) α V :
+    (∀ σ K, head_step e σ e' σ K (n, 0)) →
+    ⊢ logrel_expr V (`κ α) (fill K e') -∗ logrel_expr V (`κ α) (fill K e).
   Proof.
     intros Hpure.
     iIntros "H".
+    iIntros (κ' K') "#HK'".
     iIntros (σ) "Hs".
+    iSpecialize ("H" with "HK'").
     iSpecialize ("H" with "Hs").
     iApply (wp_wand with "H").
     iIntros (βv). iDestruct 1 as ([m m'] v σ' Hsteps) "[H2 Hs]".
-    iExists (m,m'),v,σ'. iFrame "H2 Hs".
+    iExists ((Nat.add n m),m'),v,σ'. iFrame "H2 Hs".
     iPureIntro.
-    eapply (prim_steps_app (0,0) (m,m')); eauto.
-    { eapply prim_step_steps, Hpure. }
+    eapply (prim_steps_app (n, 0) (m, m')); eauto.
+    eapply prim_step_steps.
+    rewrite !fill_comp.
+    eapply Ectx_step; last apply Hpure; done.
   Qed.
 
-  (* a matching list of closing substitutions *)
-  Inductive subs2 : scope → Type :=
-  | emp_subs2 : subs2 []
-  | cons_subs2 {S} : val [] → ITV → subs2 S → subs2 (()::S)
-  .
-
-  Equations subs_of_subs2 {S} (ss : subs2 S) : subs S [] :=
-    subs_of_subs2 emp_subs2 v => idsub v;
-    subs_of_subs2 (cons_subs2 t α ss) Vz := Val t;
-    subs_of_subs2 (cons_subs2 t α ss) (Vs v) := subs_of_subs2 ss v.
-
-  Equations its_of_subs2 {S} (ss : subs2 S) : interp_scope (E:=F) (R:=natO) S :=
-    its_of_subs2 emp_subs2 := ();
-    its_of_subs2 (cons_subs2 t α ss) := (IT_of_V α, its_of_subs2 ss).
-
-  Equations list_of_subs2 {S} (ss : subs2 S) : list (val []*ITV) :=
-    list_of_subs2 emp_subs2 := [];
-    list_of_subs2 (cons_subs2 v α ss) := (v,α)::(list_of_subs2 ss).
-
-  Lemma subs_of_emp_subs2 : subs_of_subs2 emp_subs2 ≡ idsub.
-  Proof. intros v. dependent elimination v. Qed.
-
-  Definition subs2_valid {S} (Γ : tyctx S) (ss : subs2 S) : iProp :=
-    ([∗ list] τx ∈ zip (list_of_tyctx Γ) (list_of_subs2 ss),
-      logrel_val (τx.1) (τx.2.2) (τx.2.1))%I.
-
-  Definition logrel_valid {S} (Γ : tyctx S) (e : expr S) (α : interp_scope S -n> IT) (τ : ty) : iProp :=
-    (∀ ss, subs2_valid Γ ss → logrel τ
-                                  (α (its_of_subs2 ss))
-                                  (subst_expr e (subs_of_subs2 ss)))%I.
-
-  Lemma compat_var {S} (Γ : tyctx S) (x : var S) τ :
-    typed_var Γ x τ → ⊢ logrel_valid Γ (Var x) (interp_var x) τ.
+  Lemma compat_recV {S : Set} (Γ : S -> ty) (e : expr (inc (inc S))) τ1 τ2 α :
+    ⊢ □ logrel_valid ((Γ ▹ (Tarr τ1 τ2) ▹ τ1)) e α τ2 -∗
+      logrel_valid Γ (Val $ RecV e) (interp_rec rs α) (Tarr τ1 τ2).
   Proof.
-    intros Hx. iIntros (ss) "Hss".
-    simp subst_expr.
-    iInduction Hx as [|Hx] "IH".
-    - dependent elimination ss. simp subs_of_subs2.
-      simp interp_var. rewrite /subs2_valid.
-      simp list_of_tyctx list_of_subs2 its_of_subs2. simpl.
-      iDestruct "Hss" as "[Hv Hss]".
-      iApply (logrel_of_val with "Hv").
-    - dependent elimination ss. simp subs_of_subs2.
-      simp interp_var. rewrite /subs2_valid.
-      simp list_of_tyctx list_of_subs2 its_of_subs2. simpl.
-      iDestruct "Hss" as "[Hv Hss]". by iApply "IH".
+    iIntros "#H".
+    iModIntro.
+    iIntros (ss γ) "#Hss".
+    pose (env := ss). fold env.
+    pose (f := (ir_unf rs α env)).
+    iAssert (interp_rec rs α env ≡ IT_of_V $ FunV (Next f))%I as "Hf".
+    { iPureIntro. apply interp_rec_unfold. }
+    iRewrite "Hf".
+    Opaque IT_of_V.
+    iApply logrel_of_val; term_simpl.
+    iExists _. simpl.
+    iSplit.
+    { Transparent IT_of_V. done. }
+    iModIntro.
+    iLöb as "IH". iSimpl.
+    iIntros (αv v) "#Hw".
+    rewrite APP_APP'_ITV.
+    rewrite APP_Fun.
+    rewrite laterO_map_Next.
+    rewrite -Tick_eq.
+    iIntros (κ K) "#HK".
+    iIntros (σ) "Hs".
+    rewrite hom_tick.
+    iApply wp_tick.
+    iNext.
+    unfold f.
+    Opaque extend_scope.
+    Opaque IT_of_V.
+    simpl.
+    pose (ss' := (extend_scope (extend_scope env (interp_rec rs α env)) (IT_of_V αv))).
+    pose (γ' := ((mk_subst (Val (rec bind ((γ ↑) ↑)%bind e)%syn)) ∘ ((mk_subst (shift (Val v))) ∘ ((γ ↑) ↑)%bind))%bind : inc (inc S) [⇒] ∅).
+    iSpecialize ("H" $! ss' γ' with "[]"); last first.
+    - iSpecialize ("H" $! κ K with "HK").
+      unfold ss'.
+      iSpecialize ("H" $! σ with "Hs").
+      iApply (wp_wand with "[$H] []").
+      iIntros (v') "(%m & %v'' & %σ'' & %Hstep & H)".
+      destruct m as [m m'].
+      iModIntro.
+      iExists ((Nat.add 1 m), m'), v'', σ''. iFrame "H".
+      iPureIntro.
+      eapply (prim_steps_app (1, 0) (m, m')); eauto.
+      term_simpl.
+      eapply prim_step_steps.
+      eapply Ectx_step; [reflexivity | reflexivity |].
+      subst γ'.
+      rewrite -!bind_bind_comp'.
+      econstructor.
+    - Transparent extend_scope.
+      iIntros (x'); destruct x' as [| [| x']].
+      + term_simpl.
+        iModIntro.
+        by iApply logrel_of_val.
+      + term_simpl.
+        iModIntro.
+        iRewrite "Hf".
+        iIntros (κ' K') "#HK'".
+        iApply "HK'".
+        simpl.
+        unfold logrel_arr.
+        _iExists (Next (ir_unf rs α env)).
+        iSplit; first done.
+        iModIntro.
+        iApply "IH".
+      + iModIntro.
+        subst γ'.
+        term_simpl.
+        iApply "Hss".
   Qed.
 
-  Lemma compat_if {S} (Γ : tyctx S) (e0 e1 e2 : expr S) α0 α1 α2 τ :
+  Program Definition IFSCtx_HOM α β : HOM := exist _ (λne x, IFSCtx α β x) _.
+  Next Obligation.
+    intros; simpl.
+    apply _.
+  Qed.
+
+  Program Definition HOM_compose (f g : HOM) : HOM := exist _ (`f ◎ `g) _.
+  Next Obligation.
+    intros f g; simpl.
+    apply _.
+  Qed.
+
+  Lemma compat_if {S : Set} (Γ : S -> ty) (e0 e1 e2 : expr S) α0 α1 α2 τ :
     ⊢ logrel_valid Γ e0 α0  Tnat -∗
       logrel_valid Γ e1 α1 τ -∗
       logrel_valid Γ e2 α2 τ -∗
       logrel_valid Γ (If e0 e1 e2) (interp_if rs α0 α1 α2) τ.
   Proof.
-    iIntros "H0 H1 H2". iIntros (ss) "#Hss".
-    simpl. simp subst_expr.
-    pose (s := (subs_of_subs2 ss)). fold s.
-    iSpecialize ("H0" with "Hss").
-    iApply (logrel_bind (IFSCtx (α1 (its_of_subs2 ss)) (α2 (its_of_subs2 ss)))
-              [IfCtx (subst_expr e1 s) (subst_expr e2 s)]
-                        with "H0").
-    iIntros (v βv). iDestruct 1 as (n) "[Hb ->]".
-    iRewrite "Hb". simpl.
-    unfold IFSCtx.
-    destruct (decide (0 < n)).
-    - rewrite IF_True//.
-      iSpecialize ("H1" with "Hss").
-      iApply (logrel_step_pure with "H1").
-      intros ?. apply (Ectx_step' []).
-      econstructor; eauto.
-    - rewrite IF_False; last lia.
-      iSpecialize ("H2" with "Hss").
-      iApply (logrel_step_pure with "H2").
-      intros ?. apply (Ectx_step' []).
-      econstructor; eauto. lia.
-  Qed.
-
-  Lemma compat_recV {S} Γ (e : expr (()::()::S)) τ1 τ2 α :
-    ⊢ □ logrel_valid (consC (Tarr τ1 τ2) (consC τ1 Γ)) e α τ2 -∗
-      logrel_valid Γ (Val $ RecV e) (interp_rec rs α) (Tarr τ1 τ2).
-  Proof.
-    iIntros "#H". iIntros (ss) "#Hss".
-    pose (s := (subs_of_subs2 ss)). fold s.
-    pose (env := (its_of_subs2 ss)). fold env.
-    simp subst_expr.
-    pose (f := (ir_unf rs α env)).
-    iAssert (interp_rec rs α env ≡ IT_of_V $ FunV (Next f))%I as "Hf".
-    { iPureIntro. apply interp_rec_unfold. }
-    iRewrite "Hf".
-    iApply logrel_of_val. iLöb as "IH". iSimpl.
-    iExists (Next f). iSplit; eauto.
+    iIntros "#H0 #H1 #H2".
     iModIntro.
-    iIntros (βv w) "#Hw".
-    iAssert ((APP' (Fun $ Next f) (IT_of_V βv)) ≡ (Tick (ir_unf rs α env (IT_of_V βv))))%I
-      as "Htick".
-    { iPureIntro. rewrite APP_APP'_ITV.
-      rewrite APP_Fun. simpl. done. }
-    iRewrite "Htick". iClear "Htick".
-    iIntros (σ) "Hs".
-    iApply wp_tick. iNext. simpl.
-    pose (ss' := cons_subs2 (RecV (subst_expr e (subs_lift (subs_lift s)))) (FunV (Next (ir_unf rs α env))) (cons_subs2 w βv  ss)).
-    iSpecialize ("H" $! ss' with "[Hss]").
-    { rewrite {2}/subs2_valid /ss'. simp list_of_tyctx list_of_subs2.
-      cbn-[logrel_val]. iFrame "Hss Hw". fold f. iRewrite -"Hf".
-      by iApply "IH". }
-    iSpecialize ("H"  with "Hs").
-    iClear "IH Hss Hw".
-    unfold ss'. simpl. simp its_of_subs2. fold f env.
-    iRewrite "Hf". simpl.
-    iApply (wp_wand with "H").
-    iIntros (v).
-    iDestruct 1 as ([m m'] v0  σ0 Hsteps) "[Hv Hs]".
-    iExists (1+m,0+m'),v0,σ0. iFrame "Hv Hs".
-    iPureIntro. econstructor; eauto.
-    apply (Ectx_step' []).
-    apply BetaS.
-    clear.
-    unfold subst2.
-    rewrite subst_expr_appsub.
-    apply subst_expr_proper.
-    intro v.
-    dependent elimination v.
-    { simp subs_of_subs2. unfold appsub.
-      simp subs_lift. simp subst_expr.
-      simp conssub. reflexivity. }
-    dependent elimination v.
-    { simp subs_of_subs2. unfold appsub.
-      simp subs_lift. unfold expr_lift.
-      simp ren_expr. simp subst_expr.
-      simp conssub. reflexivity. }
-    { simp subs_of_subs2. unfold appsub.
-      simp subs_lift. unfold expr_lift.
-      fold s. remember (s v) as e1.
-      rewrite ren_ren_expr.
-      rewrite subst_ren_expr.
-      trans (subst_expr e1 idsub).
-      - symmetry. apply subst_expr_idsub.
-      - apply subst_expr_proper.
-        intro v'. simpl. simp conssub.
-        reflexivity. }
-  Qed.
-
-  Lemma compat_rec {S} Γ (e : expr (()::()::S)) τ1 τ2 α :
-    ⊢ □ logrel_valid (consC (Tarr τ1 τ2) (consC τ1 Γ)) e α τ2 -∗
-      logrel_valid Γ (Rec e) (interp_rec rs α) (Tarr τ1 τ2).
-  Proof.
-    iIntros "#H". iIntros (ss) "#Hss".
-    pose (s := (subs_of_subs2 ss)). fold s.
-    pose (env := (its_of_subs2 ss)). fold env.
-    simp subst_expr.
-    iApply (logrel_step_pure (Val (RecV (subst_expr e (subs_lift (subs_lift s)))))).
-    { intros ?. eapply (Ectx_step' []). econstructor. }
-    iPoseProof (compat_recV with "H") as "H2".
-    iSpecialize ("H2" with "Hss").
-    simp subst_expr. iApply "H2".
-  Qed.
-
-  Lemma compat_app {S} Γ (e1 e2 : expr S) τ1 τ2 α1 α2 :
-  ⊢ logrel_valid Γ e1 α1 (Tarr τ1 τ2) -∗
-    logrel_valid Γ e2 α2 τ1 -∗
-    logrel_valid Γ (App e1 e2) (interp_app rs α1 α2) τ2.
-  Proof.
-    iIntros "H1 H2".  iIntros (ss) "#Hss".
-    iSpecialize ("H1" with "Hss").
-    iSpecialize ("H2" with "Hss").
-    pose (s := (subs_of_subs2 ss)). fold s.
-    pose (env := its_of_subs2 ss). fold env.
-    simp subst_expr. simpl.
-    iApply (logrel_bind (AppRSCtx (α1 env)) [AppRCtx (subst_expr e1 s)] with "H2").
-    iIntros (v2 β2) "H2". iSimpl.
-    iApply (logrel_bind (AppLSCtx (IT_of_V β2)) [AppLCtx v2] with "H1").
-    iIntros (v1 β1) "H1". simpl.
-    iDestruct "H1" as (f) "[Hα H1]".
+    iIntros (ss γ) "#Hss".
     simpl.
-    unfold AppLSCtx. iRewrite "Hα". (** XXX why doesn't simpl work here? *)
-    iApply ("H1" with "H2").
+    pose (κ' := (IFSCtx_HOM (α1 ss) (α2 ss))).
+    assert ((IF (α0 ss) (α1 ss) (α2 ss)) = ((`κ') (α0 ss))) as ->.
+    { reflexivity. }
+    term_simpl.
+    iIntros (κ K) "#HK".
+    assert ((`κ) ((IFSCtx (α1 ss) (α2 ss)) (α0 ss)) = ((`κ) ◎ (`κ')) (α0 ss)) as ->.
+    { reflexivity. }
+    pose (sss := (HOM_compose κ κ')).
+    assert ((`κ ◎ `κ') = (`sss)) as ->.
+    { reflexivity. }
+    assert (fill K (if bind γ e0 then bind γ e1 else bind γ e2)%syn = fill (ectx_compose K (IfK EmptyK (bind γ e1) (bind γ e2))) (bind γ e0)) as ->.
+    { rewrite -fill_comp.
+      reflexivity.
+    }
+    iApply (logrel_bind with "[H0] [H1 H2]").
+    - by iApply "H0".
+    - iIntros (βv v). iModIntro. iIntros "#HV".
+      term_simpl.
+      unfold logrel_nat.
+      iDestruct "HV" as "(%n & #Hn & ->)".
+      iRewrite "Hn".
+      destruct (decide (0 < n)).
+      + rewrite -fill_comp.
+        simpl.
+        unfold IFSCtx.
+        rewrite IF_True//.
+        iSpecialize ("H1" with "Hss").
+        term_simpl.
+        iSpecialize ("H1" $! κ K with "HK").
+        iIntros (σ) "Hσ".
+        iSpecialize ("H1" $! σ with "Hσ").
+        iApply (wp_wand with "[$H1] []").
+        iIntros (v) "(%m & %w & %σ' & %Hstep & H & G)".
+        iModIntro.
+        destruct m as [m m'].
+        iExists (m, m'), w, σ'. iFrame "H G".
+        iPureIntro.
+        eapply (prim_steps_app (0, 0) (m, m')); eauto.
+        eapply prim_step_steps.
+        eapply Ectx_step; [reflexivity | reflexivity |].
+        apply IfTrueS; done.
+      + rewrite -fill_comp.
+        simpl.
+        unfold IFSCtx.
+        rewrite IF_False//; last lia.
+        iSpecialize ("H2" with "Hss").
+        term_simpl.
+        iSpecialize ("H2" $! κ K with "HK").
+        iIntros (σ) "Hσ".
+        iSpecialize ("H2" $! σ with "Hσ").
+        iApply (wp_wand with "[$H2] []").
+        iIntros (v) "(%m & %w & %σ' & %Hstep & H & G)".
+        iModIntro.
+        destruct m as [m m'].
+        iExists (m, m'), w, σ'. iFrame "H G".
+        iPureIntro.
+        eapply (prim_steps_app (0, 0) (m, m')); eauto.
+        eapply prim_step_steps.
+        eapply Ectx_step; [reflexivity | reflexivity |].
+        apply IfFalseS.
+        lia.
   Qed.
 
-  Lemma compat_input {S} Γ :
-    ⊢ logrel_valid Γ (Input : expr S) (interp_input rs) Tnat.
-  Proof.
-    iIntros (ss) "Hss".
-    iIntros (σ) "Hs".
-    destruct (update_input σ) as [n σ'] eqn:Hinp.
-    iApply (wp_input with "Hs []"); first eauto.
-    iNext. iIntros "Hlc Hs".
-    iApply wp_val.
-    iExists (1,1),(Lit n),σ'.
-    iFrame "Hs". iModIntro. iSplit.
-    { iPureIntro.
-      simp subst_expr.
-      apply prim_step_steps.
-      apply (Ectx_step' []).
-      by constructor. }
-    iExists n. eauto.
-  Qed.
-  Lemma compat_output {S} Γ (e: expr S) α :
-    ⊢ logrel_valid Γ e α Tnat -∗
-      logrel_valid Γ (Output e) (interp_output rs α) Tnat.
-  Proof.
-    iIntros "H1".
-    iIntros (ss) "Hss".
-    iSpecialize ("H1" with "Hss").
-    pose (s := (subs_of_subs2 ss)). fold s.
-    pose (env := its_of_subs2 ss). fold env.
-    simp subst_expr. simpl.
-    iApply (logrel_bind (get_ret _) [OutputCtx] with "H1").
-    iIntros (v βv).
-    iDestruct 1 as (m) "[Hb ->]".
-    iRewrite "Hb". simpl.
-    iIntros (σ) "Hs".
-    rewrite get_ret_ret.
-    iApply (wp_output with "Hs []"); first done.
-    iNext. iIntros "Hlc Hs".
-    iExists (1,1),(Lit 0),_.
-    iFrame "Hs". iSplit.
-    { iPureIntro.
-      apply prim_step_steps.
-      apply (Ectx_step' []).
-      by constructor. }
-    iExists 0. eauto.
-  Qed.
+  (* Lemma compat_app {S} Γ (e1 e2 : expr S) τ1 τ2 α1 α2 : *)
+  (* ⊢ logrel_valid Γ e1 α1 (Tarr τ1 τ2) -∗ *)
+  (*   logrel_valid Γ e2 α2 τ1 -∗ *)
+  (*   logrel_valid Γ (App e1 e2) (interp_app rs α1 α2) τ2. *)
+  (* Proof. *)
+  (*   iIntros "H1 H2".  iIntros (ss) "#Hss". *)
+  (*   iSpecialize ("H1" with "Hss"). *)
+  (*   iSpecialize ("H2" with "Hss"). *)
+  (*   pose (s := (subs_of_subs2 ss)). fold s. *)
+  (*   pose (env := its_of_subs2 ss). fold env. *)
+  (*   simp subst_expr. simpl. *)
+  (*   iApply (logrel_bind (AppRSCtx (α1 env)) [AppRCtx (subst_expr e1 s)] with "H2"). *)
+  (*   iIntros (v2 β2) "H2". iSimpl. *)
+  (*   iApply (logrel_bind (AppLSCtx (IT_of_V β2)) [AppLCtx v2] with "H1"). *)
+  (*   iIntros (v1 β1) "H1". simpl. *)
+  (*   iDestruct "H1" as (f) "[Hα H1]". *)
+  (*   simpl. *)
+  (*   unfold AppLSCtx. iRewrite "Hα". (** XXX why doesn't simpl work here? *) *)
+  (*   iApply ("H1" with "H2"). *)
+  (* Qed. *)
 
-  Lemma compat_natop {S} (Γ : tyctx S) e1 e2 α1 α2 op :
-    ⊢ logrel_valid Γ e1 α1 Tnat -∗
-      logrel_valid Γ e2 α2 Tnat -∗
-      logrel_valid Γ (NatOp op e1 e2) (interp_natop rs op α1 α2) Tnat.
-  Proof.
-    iIntros "H1 H2".  iIntros (ss) "#Hss".
-    iSpecialize ("H1" with "Hss").
-    iSpecialize ("H2" with "Hss").
-    pose (s := (subs_of_subs2 ss)). fold s.
-    pose (env := its_of_subs2 ss). fold env.
-    simp subst_expr. simpl.
-    iApply (logrel_bind (NatOpRSCtx (do_natop op) (α1 env)) [NatOpRCtx op (subst_expr e1 s)] with "H2").
-    iIntros (v2 β2) "H2". iSimpl.
-    iApply (logrel_bind (NatOpLSCtx (do_natop op) (IT_of_V β2)) [NatOpLCtx op v2] with "H1").
-    iIntros (v1 β1) "H1". simpl.
-    iDestruct "H1" as (n1) "[Hn1 ->]".
-    iDestruct "H2" as (n2) "[Hn2 ->]".
-    unfold NatOpLSCtx.
-    iAssert ((NATOP (do_natop op) (IT_of_V β1) (IT_of_V β2)) ≡ Ret (do_natop op n1 n2))%I with "[Hn1 Hn2]" as "Hr".
-    { iRewrite "Hn1". simpl.
-      iRewrite "Hn2". simpl.
-      iPureIntro.
-      by rewrite NATOP_Ret. }
-    iApply (logrel_step_pure (Val (Lit (do_natop op n1 n2)))).
-    { intro. apply (Ectx_step' []). constructor.
-      destruct op; simpl; eauto. }
-    iRewrite "Hr".
-    iApply (logrel_of_val (RetV $ do_natop op n1 n2)).
-    iExists _. iSplit; eauto.
-  Qed.
+  (* Lemma compat_input {S} Γ : *)
+  (*   ⊢ logrel_valid Γ (Input : expr S) (interp_input rs) Tnat. *)
+  (* Proof. *)
+  (*   iIntros (ss) "Hss". *)
+  (*   iIntros (σ) "Hs". *)
+  (*   destruct (update_input σ) as [n σ'] eqn:Hinp. *)
+  (*   iApply (wp_input with "Hs []"); first eauto. *)
+  (*   iNext. iIntros "Hlc Hs". *)
+  (*   iApply wp_val. *)
+  (*   iExists (1,1),(Lit n),σ'. *)
+  (*   iFrame "Hs". iModIntro. iSplit. *)
+  (*   { iPureIntro. *)
+  (*     simp subst_expr. *)
+  (*     apply prim_step_steps. *)
+  (*     apply (Ectx_step' []). *)
+  (*     by constructor. } *)
+  (*   iExists n. eauto. *)
+  (* Qed. *)
+  (* Lemma compat_output {S} Γ (e: expr S) α : *)
+  (*   ⊢ logrel_valid Γ e α Tnat -∗ *)
+  (*     logrel_valid Γ (Output e) (interp_output rs α) Tnat. *)
+  (* Proof. *)
+  (*   iIntros "H1". *)
+  (*   iIntros (ss) "Hss". *)
+  (*   iSpecialize ("H1" with "Hss"). *)
+  (*   pose (s := (subs_of_subs2 ss)). fold s. *)
+  (*   pose (env := its_of_subs2 ss). fold env. *)
+  (*   simp subst_expr. simpl. *)
+  (*   iApply (logrel_bind (get_ret _) [OutputCtx] with "H1"). *)
+  (*   iIntros (v βv). *)
+  (*   iDestruct 1 as (m) "[Hb ->]". *)
+  (*   iRewrite "Hb". simpl. *)
+  (*   iIntros (σ) "Hs". *)
+  (*   rewrite get_ret_ret. *)
+  (*   iApply (wp_output with "Hs []"); first done. *)
+  (*   iNext. iIntros "Hlc Hs". *)
+  (*   iExists (1,1),(Lit 0),_. *)
+  (*   iFrame "Hs". iSplit. *)
+  (*   { iPureIntro. *)
+  (*     apply prim_step_steps. *)
+  (*     apply (Ectx_step' []). *)
+  (*     by constructor. } *)
+  (*   iExists 0. eauto. *)
+  (* Qed. *)
 
-  Lemma fundamental {S} (Γ : tyctx S) τ e :
+  (* Lemma compat_natop {S} (Γ : tyctx S) e1 e2 α1 α2 op : *)
+  (*   ⊢ logrel_valid Γ e1 α1 Tnat -∗ *)
+  (*     logrel_valid Γ e2 α2 Tnat -∗ *)
+  (*     logrel_valid Γ (NatOp op e1 e2) (interp_natop rs op α1 α2) Tnat. *)
+  (* Proof. *)
+  (*   iIntros "H1 H2".  iIntros (ss) "#Hss". *)
+  (*   iSpecialize ("H1" with "Hss"). *)
+  (*   iSpecialize ("H2" with "Hss"). *)
+  (*   pose (s := (subs_of_subs2 ss)). fold s. *)
+  (*   pose (env := its_of_subs2 ss). fold env. *)
+  (*   simp subst_expr. simpl. *)
+  (*   iApply (logrel_bind (NatOpRSCtx (do_natop op) (α1 env)) [NatOpRCtx op (subst_expr e1 s)] with "H2"). *)
+  (*   iIntros (v2 β2) "H2". iSimpl. *)
+  (*   iApply (logrel_bind (NatOpLSCtx (do_natop op) (IT_of_V β2)) [NatOpLCtx op v2] with "H1"). *)
+  (*   iIntros (v1 β1) "H1". simpl. *)
+  (*   iDestruct "H1" as (n1) "[Hn1 ->]". *)
+  (*   iDestruct "H2" as (n2) "[Hn2 ->]". *)
+  (*   unfold NatOpLSCtx. *)
+  (*   iAssert ((NATOP (do_natop op) (IT_of_V β1) (IT_of_V β2)) ≡ Ret (do_natop op n1 n2))%I with "[Hn1 Hn2]" as "Hr". *)
+  (*   { iRewrite "Hn1". simpl. *)
+  (*     iRewrite "Hn2". simpl. *)
+  (*     iPureIntro. *)
+  (*     by rewrite NATOP_Ret. } *)
+  (*   iApply (logrel_step_pure (Val (Lit (do_natop op n1 n2)))). *)
+  (*   { intro. apply (Ectx_step' []). constructor. *)
+  (*     destruct op; simpl; eauto. } *)
+  (*   iRewrite "Hr". *)
+  (*   iApply (logrel_of_val (RetV $ do_natop op n1 n2)). *)
+  (*   iExists _. iSplit; eauto. *)
+  (* Qed. *)
+
+  (* TODO: boring cases + callcc + throw *)
+  Lemma fundamental {S : Set} (Γ : S -> ty) τ e :
     typed Γ e τ → ⊢ logrel_valid Γ e (interp_expr rs e) τ
-  with fundamental_val {S} (Γ : tyctx S) τ v :
+  with fundamental_val {S : Set} (Γ : S -> ty) τ v :
     typed_val Γ v τ → ⊢ logrel_valid Γ (Val v) (interp_val rs v) τ.
   Proof.
-    - induction 1; simpl.
-      + by apply fundamental_val.
-      + by apply compat_var.
-      + iApply compat_rec. iApply IHtyped.
-      + iApply compat_app.
-        ++ iApply IHtyped1.
-        ++ iApply IHtyped2.
-      + iApply compat_natop.
-        ++ iApply IHtyped1.
-        ++ iApply IHtyped2.
-      + iApply compat_if.
-        ++ iApply IHtyped1.
-        ++ iApply IHtyped2.
-        ++ iApply IHtyped3.
-      + iApply compat_input.
-      + iApply compat_output.
-        iApply IHtyped.
-    - induction 1; simpl.
-      + iIntros (ss) "Hss". simp subst_expr. simpl.
-        iApply (logrel_of_val (RetV n)). iExists n. eauto.
-      + iApply compat_recV. by iApply fundamental.
-  Qed.
+  Admitted.
+  (* - induction 1; simpl. *)
+  (*   + by apply fundamental_val. *)
+  (*   + by apply compat_var. *)
+  (*   + iApply compat_rec. iApply IHtyped. *)
+  (*   + iApply compat_app. *)
+  (*     ++ iApply IHtyped1. *)
+  (*     ++ iApply IHtyped2. *)
+  (*   + iApply compat_natop. *)
+  (*     ++ iApply IHtyped1. *)
+  (*     ++ iApply IHtyped2. *)
+  (*   + iApply compat_if. *)
+  (*     ++ iApply IHtyped1. *)
+  (*     ++ iApply IHtyped2. *)
+  (*     ++ iApply IHtyped3. *)
+  (*   + iApply compat_input. *)
+  (*   + iApply compat_output. *)
+  (*     iApply IHtyped. *)
+  (* - induction 1; simpl. *)
+  (*   + iIntros (ss) "Hss". simp subst_expr. simpl. *)
+  (*     iApply (logrel_of_val (RetV n)). iExists n. eauto. *)
+  (*   + iApply compat_recV. by iApply fundamental. *)
+  (* Qed. *)
 
 End logrel.
 
 Definition κ {S} {E} : ITV E natO → val S :=  λ x,
     match x with
-    | core.RetV n => Lit n
-    | _ => Lit 0
+    | core.RetV n => LitV n
+    | _ => LitV 0
     end.
-Lemma κ_Ret {S} {E} n : κ ((RetV n) : ITV E natO) = (Lit n : val S).
+Lemma κ_Ret {S} {E} n : κ ((RetV n) : ITV E natO) = (LitV n : val S).
 Proof.
   Transparent RetV. unfold RetV. simpl. done. Opaque RetV.
 Qed.
 Definition rs : gReifiers 1 := gReifiers_cons reify_io gReifiers_nil.
 
+Require Import gitrees.gitree.greifiers.
+
 Lemma logrel_nat_adequacy  Σ `{!invGpreS Σ}`{!statePreG rs natO Σ} {S} (α : IT (gReifiers_ops rs) natO) (e : expr S) n σ σ' k :
   (∀ `{H1 : !invGS Σ} `{H2: !stateG rs natO Σ},
       (True ⊢ logrel rs Tnat α e)%I) →
-  ssteps (gReifiers_sReifier rs) α (σ,()) (Ret n) σ' k → ∃ m σ', prim_steps e σ (Val $ Lit n) σ' m.
+  ssteps (gReifiers_sReifier rs) α (σ,()) (Ret n) σ' k → ∃ m σ', prim_steps e σ (Val $ LitV n) σ' m.
 Proof.
   intros Hlog Hst.
   pose (ϕ := λ (βv : ITV (gReifiers_ops rs) natO),
@@ -423,8 +562,8 @@ Proof.
     exists m', σ2. revert Hm. by rewrite κ_Ret. }
   eapply (wp_adequacy 0); eauto.
   intros Hinv1 Hst1.
-  pose (Φ := (λ (βv : ITV (gReifiers_ops rs) natO), ∃ n, logrel_val rs Tnat (Σ:=Σ) (S:=S) βv (Lit n)
-          ∗ ⌜∃ m σ', prim_steps e σ (Val $ Lit n) σ' m⌝)%I).
+  pose (Φ := (λ (βv : ITV (gReifiers_ops rs) natO), ∃ n, logrel_val rs Tnat (Σ:=Σ) (S:=S) βv (LitV n)
+          ∗ ⌜∃ m σ', prim_steps e σ (Val $ LitV n) σ' m⌝)%I).
   assert (NonExpansive Φ).
   { unfold Φ.
     intros l a1 a2 Ha. repeat f_equiv. done. }
@@ -445,9 +584,9 @@ Proof.
   iPoseProof (Hlog with "[//]") as "Hlog".
   iAssert (has_substate σ) with "[Hs]" as "Hs".
   { unfold has_substate, has_full_state.
-    assert (of_state rs (IT (gReifiers_ops rs) natO) (σ, ()) ≡
-            of_idx rs (IT (gReifiers_ops rs) natO) sR_idx (sR_state σ)) as -> ; last done. 
-    intro j. unfold sR_idx. simpl.
+    assert ((of_state rs (IT (sReifier_ops (gReifiers_sReifier rs)) natO) (σ, ())) ≡
+            (of_idx rs (IT (sReifier_ops (gReifiers_sReifier rs)) natO) sR_idx (sR_state σ))) as -> ; last done.
+    intros j. unfold sR_idx. simpl.
     unfold of_state, of_idx.
     destruct decide as [Heq|]; last first.
     { inv_fin j; first done.
@@ -456,6 +595,18 @@ Proof.
     intros Heq.
     rewrite (eq_pi _ _ Heq eq_refl)//.
   }
+  unshelve epose (idHOM := _ : (HOM rs)).
+  { exists idfun. apply IT_hom_idfun. }
+  iSpecialize ("Hlog" $! idHOM EmptyK with "[]").
+  { iIntros (βv v); iModIntro. iIntros "Hv". iIntros (σ'') "HS".
+    iApply wp_val.
+    iModIntro.
+    iExists (0, 0), v, σ''.
+    iSplit; first iPureIntro.
+    - apply prim_steps_zero.
+    - by iFrame.
+  }
+  simpl.
   iSpecialize ("Hlog" $! σ with "Hs").
   iApply (wp_wand with"Hlog").
   iIntros ( βv). iIntros "H".
@@ -465,24 +616,25 @@ Proof.
   iExists l. iSplit; eauto.
 Qed.
 
+Program Definition ı_scope : @interp_scope (gReifiers_ops rs) natO _ Empty_set := λne (x : ∅), match x with end.
 
-Theorem adequacy (e : expr []) (k : nat) σ σ' n :
-  typed empC e Tnat →
-  ssteps (gReifiers_sReifier rs) (interp_expr rs e ()) (σ,()) (Ret k : IT _ natO) σ' n →
-  ∃ mm σ', prim_steps e σ (Val $ Lit k) σ' mm.
+Theorem adequacy (e : expr ∅) (k : nat) σ σ' n :
+  typed □ e Tnat →
+  ssteps (gReifiers_sReifier rs) (interp_expr rs e ı_scope) (σ,()) (Ret k : IT _ natO) σ' n →
+  ∃ mm σ', prim_steps e σ (Val $ LitV k) σ' mm.
 Proof.
   intros Hty Hst.
   pose (Σ:=#[invΣ;stateΣ rs natO]).
-  eapply (logrel_nat_adequacy Σ (interp_expr rs e ())); last eassumption.
+  eapply (logrel_nat_adequacy Σ (interp_expr rs e ı_scope)); last eassumption.
   intros ? ?.
   iPoseProof (fundamental rs) as "H".
   { apply Hty. }
   unfold logrel_valid.
   iIntros "_".
-  iSpecialize ("H" $! (emp_subs2 rs)).
-  simp its_of_subs2.
-  rewrite subs_of_emp_subs2.
-  rewrite subst_expr_idsub.
+  unshelve iSpecialize ("H" $! ı_scope _ with "[]").
+  { apply ı%bind. }
+  { iIntros (x); destruct x. }
+  rewrite ebind_id; first last.
+  { intros ?; reflexivity. }
   iApply "H".
-  unfold subs2_valid. done.
 Qed.
