theories/lang_generic_sem.v
@@ -27,9 +27,12 @@ Section interp.
   Global Instance interp_var_proper {S : Set} (v : S) : Proper ((≡) ==> (≡)) (interp_var v).
   Proof. apply ne_proper. apply _. Qed.
 
-  (* TODO: rewrite in normal-human-being style *)
   Program Definition extend_scope {S : Set}  : interp_scope S -n> IT -n> interp_scope (inc S)
-    := λne γ μ x, let x' : inc S := x in match x' with | VZ => μ | VS x'' => γ x'' end.
+    := λne γ μ x, let x' : inc S := x in
+                  match x' with
+                  | VZ => μ
+                  | VS x'' => γ x''
+                  end.
   Next Obligation.
     match goal with
     | H : context G [(inc S)] |- _ => revert H
@@ -46,37 +49,6 @@ Section interp.
   Program Definition ren_scope {S S'} (δ : S [→] S') (env : interp_scope S')
     : interp_scope S := λne x, env (δ x).
 
-  (* (** scope substituions *) *)
-  (* Inductive ssubst : Set → Type := *)
-  (* | emp_ssubst : ssubst ∅ *)
-  (* | cons_ssubst {S} : ITV → ssubst S → ssubst (inc S) *)
-  (* . *)
-
-  (* Equations interp_ssubst {S} (ss : ssubst S) : interp_scope S := *)
-  (*   interp_ssubst emp_ssubst := tt; *)
-  (*   interp_ssubst (cons_ssubst αv ss) := (IT_of_V αv, interp_ssubst ss). *)
-
-  (* Equations list_of_ssubst {S} (ss : ssubst S) : list ITV := *)
-  (*   list_of_ssubst emp_ssubst := []; *)
-  (*   list_of_ssubst (cons_ssubst αv ss) := αv::(list_of_ssubst ss). *)
-
-  (* Equations ssubst_split {S1 S2} (αs : ssubst (S1++S2)) : ssubst S1 * ssubst S2 := *)
-  (*   ssubst_split (S1:=[]) αs := (emp_ssubst,αs); *)
-  (*   ssubst_split (S1:=u::_) (cons_ssubst αv αs) := *)
-  (*     (cons_ssubst αv (ssubst_split αs).1, (ssubst_split αs).2). *)
-  (* Lemma interp_scope_ssubst_split {S1 S2} (αs : ssubst (S1++S2)) : *)
-  (*   interp_scope_split (interp_ssubst αs) ≡ *)
-  (*     (interp_ssubst (ssubst_split αs).1, interp_ssubst (ssubst_split αs).2). *)
-  (* Proof. *)
-  (*   induction S1 as [|u S1]; simpl. *)
-  (*   - simp ssubst_split. simpl. *)
-  (*     simp interp_ssubst. done. *)
-  (*   - dependent elimination αs as [cons_ssubst αv αs]. *)
-  (*     simp ssubst_split. simpl. *)
-  (*     simp interp_ssubst. repeat f_equiv; eauto; simpl. *)
-  (*      + rewrite IHS1//. *)
-  (*      + rewrite IHS1//. *)
-  (* Qed. *)
 End interp.
 
 (* Common definitions and lemmas for Kripke logical relations *)
@@ -94,43 +66,55 @@ Section kripke_logrel.
   Notation iProp := (iProp Σ).
 
   Context {A:ofe}. (* The type & predicate for the explicit Kripke worlds *)
-  Variable (P : A → iProp).
-  Context `{!NonExpansive P}.
+  Variable (P : A -n> iProp).
 
   Implicit Types α β : IT.
   Implicit Types αv βv : ITV.
   Implicit Types Φ Ψ : ITV -n> iProp.
 
   Program Definition expr_pred (α : IT) (Φ : ITV -n> iProp) : iProp :=
-    (∀ x : A, P x -∗ WP@{rs} α @ s {{ v, ∃ y : A, Φ v ∗ P y }}).
-  #[export] Instance expr_pred_ne : NonExpansive2 expr_pred.
-  Proof. solve_proper. Qed.
-  #[export] Instance expr_pred_proper : Proper ((≡) ==> (≡) ==> (≡)) expr_pred .
-  Proof. solve_proper. Qed.
+    (∀ x : A, P x -∗ wp rs α s ⊤ (λne v, ∃ y : A, Φ v ∗ P y)).
+  Next Obligation.
+    solve_proper.
+  Qed.
+
+  (* #[export] Instance expr_pred_ne : NonExpansive2 expr_pred. *)
+  (* Proof. *)
+  (*   solve_proper_prepare. *)
+  (*   f_equiv. *)
+  (*   intro; simpl. *)
+  (*   f_equiv. *)
+  (*   rewrite clwp_eq. *)
+    
+  (*   apply clwp_ne'''. *)
+  (* Qed. *)
+  (* #[export] Instance expr_pred_proper : Proper ((≡) ==> (≡) ==> (≡)) expr_pred . *)
+  (* Proof. solve_proper. Qed. *)
 
   Lemma expr_pred_ret α αv Φ `{!IntoVal α αv} :
     Φ αv ⊢ expr_pred α Φ.
   Proof.
     iIntros "H".
     iIntros (x) "Hx". iApply wp_val.
-    eauto with iFrame.
+    simpl.
+    iExists x.
+    by iFrame.    
   Qed.
 
-  Lemma expr_pred_bind f `{!IT_hom f} α Φ Ψ `{!NonExpansive Φ} :
-    expr_pred α Ψ ⊢
-    (∀ αv, Ψ αv -∗ expr_pred (f (IT_of_V αv)) Φ) -∗
-    expr_pred (f α) Φ.
-  Proof.
-    iIntros "H1 H2".
-    iIntros (x) "Hx".
-    iApply wp_bind.
-    { solve_proper. }
-    iSpecialize ("H1" with "Hx").
-    iApply (wp_wand with "H1").
-    iIntros (βv). iDestruct 1 as (y) "[Hb Hy]".
-    iModIntro.
-    iApply ("H2" with "Hb Hy").
-  Qed.
+  (* Lemma expr_pred_bind (f : IT -n> IT) {Hf : IT_hom f} α (Φ Ψ : ITV -n> iProp) : *)
+  (*   expr_pred α Ψ ⊢ *)
+  (*   (∀ αv, Ψ αv -∗ expr_pred (f (IT_of_V αv)) Φ) -∗ *)
+  (*   expr_pred (f α) Φ. *)
+  (* Proof. *)
+  (*   iIntros "H1 H2". *)
+  (*   iIntros (x) "Hx". *)
+  (*   unshelve iApply clwp_bind; first done. *)
+  (*   iSpecialize ("H1" with "Hx"). *)
+  (*   iApply (clwp_wand with "H1"). *)
+  (*   iIntros (βv). iDestruct 1 as (y) "[Hb Hy]". *)
+  (*   simpl. *)
+  (*   iApply ("H2" with "Hb Hy"). *)
+  (* Qed. *)
 
   Lemma expr_pred_frame α Φ :
     WP@{rs} α @ s {{ Φ }} ⊢ expr_pred α Φ.
@@ -138,9 +122,12 @@ Section kripke_logrel.
     iIntros "H".
     iIntros (x) "Hx".
     iApply (wp_wand with "H").
-    eauto with iFrame.
+    simpl.
+    iIntros (v) "Hv".
+    iExists x.
+    by iFrame.
   Qed.
 
 End kripke_logrel.
 
-Arguments expr_pred_bind {_ _ _ _ _ _ _ _ _ _} f {_}.
+(* Arguments expr_pred_bind {_ _ _ _ _ _ _ _ _ _} f {_}. *)
